src/proofs/no_slashable_attestations/supporting_lemmas/ind_inv_implies_safety/ind_inv_implies_safety.dfy
@@ -1,0 +1,102 @@
+include "../../../../common/commons.dfy"
+include "../../common/attestation_creation_instrumented.dfy"
+include "../../../../specs/consensus/consensus.dfy"
+include "../../../../specs/network/network.dfy"
+include "../../../../specs/dv/dv_attestation_creation.dfy"
+include "../../../../specs/dvc/dvc_attestation_creation.dfy"
+
+include "../../../common/helper_sets_lemmas.dfy"
+include "../../../no_slashable_attestations/common/common_proofs.dfy"
+include "../../../no_slashable_attestations/common/dvc_spec_axioms.dfy"
+
+include "../dv_next_preserves_ind_inv/proofs_intermediate_steps.dfy"
+include "../dv_next_preserves_ind_inv/ind_inv_dv_next.dfy"
+
+include "../inv.dfy"
+include "../ind_inv.dfy"
+
+include "core_proofs.dfy"
+
+
+module Ind_Inv_Implies_Safety
+{
+    import opened Types 
+    import opened CommonFunctions
+    import opened ConsensusSpec
+    import opened NetworkSpec
+    import opened DVC_Spec
+    import opened DV
+    import opened Att_Ind_Inv_With_Empty_Init_Att_Slashing_DB
+    import opened Att_Inv_With_Empty_Initial_Attestation_Slashing_DB
+    
+    import opened Core_Proofs
+    import opened Ind_Inv_DV_Next
+    import opened Proofs_Intermediate_Steps
+
+    lemma lemma_ind_inv_dv_ind(dv: DVState, dv': DVState)       
+    requires DV.NextPreCond(dv)
+    requires DV.Next(dv, dv')  
+    requires ind_inv(dv)    
+    ensures ind_inv(dv')  
+    ensures DV.NextPreCond(dv')
+    {
+        var e :|
+            && validEvent(dv, e)
+            && NextEvent(dv, e, dv');
+
+        lemma_ind_inv_dv_next_ind_inv(dv, e, dv');
+        lemma_NextPreCond(dv');
+    }      
+
+    predicate non_slashable_attestations(
+        dv: DVState
+    )
+    {
+        forall a: Attestation, a': Attestation
+                | 
+                && a in dv.all_attestations_created
+                && is_valid_attestation(a, dv.dv_pubkey)
+                && a' in dv.all_attestations_created
+                && is_valid_attestation(a', dv.dv_pubkey)     
+                ::
+                && !is_slashable_attestation_data_eth_spec(a.data, a'.data)
+                && !is_slashable_attestation_data_eth_spec(a'.data, a.data)
+    }
+
+    lemma lemma_ind_inv_no_slashable_submitted_attestations(dv: DVState)
+    requires ind_inv(dv)    
+    ensures non_slashable_attestations(dv)
+    {   
+        lemma_ind_inv_implies_intermediate_steps(dv);
+
+        forall a: Attestation, a': Attestation
+                    | 
+                    && a in dv.all_attestations_created
+                    && is_valid_attestation(a, dv.dv_pubkey)
+                    && a' in dv.all_attestations_created
+                    && is_valid_attestation(a', dv.dv_pubkey)     
+        ensures && !is_slashable_attestation_data_eth_spec(a.data, a'.data)
+                && !is_slashable_attestation_data_eth_spec(a'.data, a.data);
+        {
+            assert 
+            && inv_quorum_constraints(dv)
+            && inv_unchanged_honesty(dv)
+            && concl_exists_honest_dvc_that_sent_att_share_for_submitted_att(dv)
+            && pred_data_of_att_share_is_decided_value(dv)
+            && inv_decided_value_of_consensus_instance_is_decided_by_quorum(dv)    
+            && inv_sent_validity_predicate_is_based_on_rcvd_duty_and_slashing_db_in_hist(dv)
+            && inv_db_of_validity_predicate_contains_all_previous_decided_values(dv)
+            && a in dv.all_attestations_created
+            && is_valid_attestation(a, dv.dv_pubkey)
+            && a' in dv.all_attestations_created
+            && is_valid_attestation(a', dv.dv_pubkey)
+            && inv_sent_validity_predicate_only_for_slots_stored_in_att_slashing_db_hist(dv)
+            && inv_all_validity_predicates_are_stored_in_att_slashing_db_hist(dv)
+            && inv_queued_att_duty_is_rcvd_duty0(dv)
+            && inv_queued_att_duty_is_rcvd_duty1(dv)
+            ;
+            lemma_no_slashable_submitted_attestations(dv, a, a');
+        }
+    }
+
+}
